progress on teleport, rewriting for equivalences

Teleport.v
@@ -1,6 +1,8 @@
 Require Import SQIMP.
 Require Import UnitarySem.
 
+Module UTeleport.
+
 Definition bell (c b : nat) : ucom := H c ; CNOT c b.
 Definition alice (a c : nat) : ucom := CNOT a c ; H a.
 Definition bob (a c b: nat) : ucom := CNOT c b; CZ a b.
@@ -55,3 +57,327 @@ Proof.
   all : rewrite <- (Cmult_assoc (/2) _ _); autorewrite with C_db; reflexivity.
 Qed.
 
+End UTeleport.
+
+Section NDTeleport.
+
+Definition q := 0. (* qubit for transmission *)
+Definition a := 1. (* alice's qubit *)
+Definition b := 2. (* bob's qubit *)
+
+Require Import NDSem.
+
+Definition bell : com := H a ; CNOT a b.
+Definition alice : com := CNOT q a ; H a ; meas q ; meas a.
+Definition bob : com := CNOT q b; CZ q a; reset q; reset a.
+Definition teleport : com := bell; alice; bob.
+
+Open Scope R_scope.
+
+Definition epr00 : Vector 4 := / √ 2 .* ∣ 0, 0 ⟩ .+ / √ 2 .* ∣ 1, 1 ⟩.
+
+Definition notc : Matrix 4 4 :=
+  fun x y => match x, y with 
+          | 1, 3 => 1%C
+          | 3, 1 => 1%C
+          | 0, 0 => 1%C
+          | 2, 2 => 1%C
+          | _, _ => 0%C
+          end.          
+
+Lemma cnot_decomposition : ∣1⟩⟨1∣ ⊗ σx .+ ∣0⟩⟨0∣ ⊗ I 2 = cnot.
+Proof. solve_matrix. Qed.                                               
+
+Lemma notc_decomposition : σx ⊗ ∣1⟩⟨1∣ .+ I 2 ⊗ ∣0⟩⟨0∣ = notc.
+Proof. solve_matrix. Qed.                                               
+
+Require Import Dirac.
+
+Ltac kmp_rewrite A B C D :=
+  rewrite (kron_mixed_product' _ _ _ _ _ _ _ _ _ _ _ A B C D); simpl; unify_pows_two; try omega.
+
+Ltac destruct_seqs := 
+  repeat match goal with
+  | [H : ?a / _ ⇩ _ |- _] => unfold a in H
+  | [H : (_ ; _) / _ ⇩ _ |- _] => dependent destruction H
+  end.
+
+Ltac destruct_apps := 
+  repeat match goal with
+  | [H : app _ _ / _ ⇩ _ |- _] => dependent destruction H
+  end.
+
+(* Thought I had this. *)
+(* Generalizable? *)
+Lemma ket_decomposition : forall (ψ : Vector 2), 
+  WF_Matrix _ _ ψ ->
+  ψ = (ψ 0%nat 0%nat) .* ∣ 0 ⟩ .+ (ψ 1%nat 0%nat) .* ∣ 1 ⟩.
+Proof.
+  intros.
+  prep_matrix_equality.
+  unfold scale, Mplus.
+  destruct y as [|y']. 
+  2:{ rewrite H; try omega. 
+      unfold ket, qubit0, qubit1. simpl. 
+      repeat (destruct x; try clra). 
+  }
+  destruct x as [| [| n]]; unfold ket, qubit0, qubit1; simpl; try clra.  
+  rewrite H; try omega.
+  clra.
+Qed. 
+
+Notation "∣+⟩" := (1/√2 .* ∣0⟩ .+ 1/√2 .* ∣1⟩)%C.
+Notation "∣-⟩" := (1/√2 .* ∣0⟩ .+ (- 1/√2) .* ∣1⟩)%C.
+
+Definition mult' := mult.
+Definition pow' := Nat.pow.
+Lemma mult_lock : mult = mult'. reflexivity. Qed.
+Lemma pow_lock : Nat.pow = pow'. reflexivity. Qed.
+Opaque mult'.
+Opaque pow'.
+
+(* Simplifies without simplifying Matrix dimensions. *)
+Ltac simpl' := 
+  repeat rewrite Nat.pow_1_r in *;
+  repeat rewrite pow_lock;
+  repeat rewrite mult_lock;
+  simpl;
+  repeat rewrite <- mult_lock;
+  repeat rewrite <- pow_lock.
+
+(* Normalize: Gives default dimensions to matrix expressions *)
+Ltac restore_dims :=
+  repeat match goal with
+  | [ |- context[@Mmult ?m ?n ?o ?A ?B]] => let Matrix m' n' := type of A in 
+                                          let Matrix n'' o' := type of B in 
+                                          replace m with m' by easy
+         end.
+
+
+
+Lemma teleport_correct : forall (ψ : Vector (2^1)) (ψ' : Vector (2^3)),
+  WF_Matrix _ _ ψ ->
+  teleport / (ψ  ⊗ ∣ 0 , 0 ⟩) ⇩ ψ' -> ψ' = ∣ 0 , 0 ⟩ ⊗ ψ.   
+Proof.
+  intros ψ ψ' WF H.
+  destruct_seqs; destruct_apps.
+  evar (e : Vector (2^3)).  
+  assert ((ueval 3 U_H [a] × (ueval 3 U_CNOT (q::[a]) × (ueval 3 U_CNOT (a::[b]) × (ueval 3 U_H [a] × (ψ ⊗ ∣ 0, 0 ⟩))))) = e).
+  rewrite (ket_decomposition ψ); auto.
+  unfold ueval, ueval_cnot, ueval1, pad; simpl'; Msimpl.
+  setoid_rewrite cnot_decomposition.
+  autorewrite with ket_db.
+  rewrite <- kron_assoc.
+  rewrite <- kron_assoc.
+  Msimpl'.
+setoid_rewrite kron_mixed_product'.
+  Set Printing All.
+
+  rewrite kron_mixed_product'.
+  Msimpl.
+  Msimpl'.
+  autorewrite with ket_db.
+  setoid_rewrite (kron_assoc _ _ _ _ _ _ ∣ 0 ⟩ ∣ 0 ⟩ ∣ 0 ⟩).
+  setoid_rewrite (kron_assoc _ _ _ _ _ _ ∣ 0 ⟩ ∣ 1 ⟩ ∣ 0 ⟩).
+  setoid_rewrite (kron_assoc _ _ _ _ _ _ ∣ 1 ⟩ ∣ 0 ⟩ ∣ 0 ⟩).
+  setoid_rewrite (kron_assoc _ _ _ _ _ _ ∣ 1 ⟩ ∣ 1 ⟩ ∣ 0 ⟩).
+  Msimpl'; try reflexivity.
+  autorewrite with ket_db.
+  setoid_rewrite CNOT00_spec.
+  setoid_rewrite CNOT10_spec.
+  setoid_rewrite <- (kron_assoc _ _ _ _ _ _ ∣ 0 ⟩ ∣ 0 ⟩ ∣ 0 ⟩).
+  setoid_rewrite <- (kron_assoc _ _ _ _ _ _ ∣ 0 ⟩ ∣ 1 ⟩ ∣ 1 ⟩).
+  setoid_rewrite <- (kron_assoc _ _ _ _ _ _ ∣ 1 ⟩ ∣ 0 ⟩ ∣ 0 ⟩).
+  setoid_rewrite <- (kron_assoc _ _ _ _ _ _ ∣ 1 ⟩ ∣ 1 ⟩ ∣ 1 ⟩).
+  Msimpl'. simpl. 
+  kmp_rewrite cnot (I 2) ∣ 0 , 0 ⟩ ∣ 0 ⟩.
+  kmp_rewrite cnot (I 2) ∣ 0 , 1 ⟩ ∣ 1 ⟩.
+  kmp_rewrite cnot (I 2) ∣ 1 , 0 ⟩ ∣ 0 ⟩.
+  kmp_rewrite cnot (I 2) ∣ 1 , 1 ⟩ ∣ 1 ⟩.
+  autorewrite with ket_db; auto with wf_db.
+  setoid_rewrite CNOT00_spec.
+  setoid_rewrite CNOT01_spec.
+  setoid_rewrite CNOT10_spec.
+  setoid_rewrite CNOT11_spec.
+  kmp_rewrite (I 2 ⊗ hadamard) (I 2) ∣ 0 , 0 ⟩ ∣ 0 ⟩.
+  kmp_rewrite (I 2 ⊗ hadamard) (I 2) ∣ 0 , 1 ⟩ ∣ 1 ⟩.
+  kmp_rewrite (I 2 ⊗ hadamard) (I 2) ∣ 1 , 1 ⟩ ∣ 0 ⟩.
+  kmp_rewrite (I 2 ⊗ hadamard) (I 2) ∣ 1 , 0 ⟩ ∣ 1 ⟩.
+  Msimpl'; trivial.
+  autorewrite with ket_db C_db.  
+  kmp_rewrite cnot (I 2) ∣ 0 , 1 ⟩ ∣ 1 ⟩.
+  kmp_rewrite cnot (I 2) ∣ 1 , 0 ⟩ ∣ 0 ⟩.
+  kmp_rewrite cnot (I 2) ∣ 1 , 1 ⟩ ∣ 1 ⟩.
+
+
+Lemma teleport_correct : forall (ψ : Vector (2^1)) (ψ' : Vector (2^3)),
+  WF_Matrix _ _ ψ ->
+  teleport / (ψ  ⊗ ∣ 0 , 0 ⟩) ⇩ ψ' -> ψ' = ∣ 0 , 0 ⟩ ⊗ ψ.   
+Proof.
+  intros ψ ψ' WF H.
+  destruct_seqs; destruct_apps.
+  evar (e : Vector (2^3)).  
+  assert ((ueval 3 U_H [a] × (ueval 3 U_CNOT (q::[a]) × (ueval 3 U_CNOT (a::[b]) × (ueval 3 U_H [a] × (ψ ⊗ ∣ 0, 0 ⟩))))) = e).
+  rewrite (ket_decomposition ψ); auto.
+  unfold ueval, ueval_cnot, ueval1, pad; simpl; Msimpl.
+  setoid_rewrite cnot_decomposition.
+  autorewrite with ket_db.
+  setoid_rewrite <- (kron_assoc _ _ _ _ _ _ ∣ 0 ⟩ ∣ 0 ⟩ ∣ 0 ⟩).
+  setoid_rewrite <- (kron_assoc _ _ _ _ _ _ ∣ 1 ⟩ ∣ 0 ⟩ ∣ 0 ⟩).
+  Msimpl'; try reflexivity.
+  autorewrite with ket_db.
+  setoid_rewrite (kron_assoc _ _ _ _ _ _ ∣ 0 ⟩ ∣ 0 ⟩ ∣ 0 ⟩).
+  setoid_rewrite (kron_assoc _ _ _ _ _ _ ∣ 0 ⟩ ∣ 1 ⟩ ∣ 0 ⟩).
+  setoid_rewrite (kron_assoc _ _ _ _ _ _ ∣ 1 ⟩ ∣ 0 ⟩ ∣ 0 ⟩).
+  setoid_rewrite (kron_assoc _ _ _ _ _ _ ∣ 1 ⟩ ∣ 1 ⟩ ∣ 0 ⟩).
+  Msimpl'; try reflexivity.
+  autorewrite with ket_db.
+  setoid_rewrite CNOT00_spec.
+  setoid_rewrite CNOT10_spec.
+  setoid_rewrite <- (kron_assoc _ _ _ _ _ _ ∣ 0 ⟩ ∣ 0 ⟩ ∣ 0 ⟩).
+  setoid_rewrite <- (kron_assoc _ _ _ _ _ _ ∣ 0 ⟩ ∣ 1 ⟩ ∣ 1 ⟩).
+  setoid_rewrite <- (kron_assoc _ _ _ _ _ _ ∣ 1 ⟩ ∣ 0 ⟩ ∣ 0 ⟩).
+  setoid_rewrite <- (kron_assoc _ _ _ _ _ _ ∣ 1 ⟩ ∣ 1 ⟩ ∣ 1 ⟩).
+  Msimpl'. simpl. 
+  kmp_rewrite cnot (I 2) ∣ 0 , 0 ⟩ ∣ 0 ⟩.
+  kmp_rewrite cnot (I 2) ∣ 0 , 1 ⟩ ∣ 1 ⟩.
+  kmp_rewrite cnot (I 2) ∣ 1 , 0 ⟩ ∣ 0 ⟩.
+  kmp_rewrite cnot (I 2) ∣ 1 , 1 ⟩ ∣ 1 ⟩.
+  autorewrite with ket_db; auto with wf_db.
+  setoid_rewrite CNOT00_spec.
+  setoid_rewrite CNOT01_spec.
+  setoid_rewrite CNOT10_spec.
+  setoid_rewrite CNOT11_spec.
+  kmp_rewrite (I 2 ⊗ hadamard) (I 2) ∣ 0 , 0 ⟩ ∣ 0 ⟩.
+  kmp_rewrite (I 2 ⊗ hadamard) (I 2) ∣ 0 , 1 ⟩ ∣ 1 ⟩.
+  kmp_rewrite (I 2 ⊗ hadamard) (I 2) ∣ 1 , 1 ⟩ ∣ 0 ⟩.
+  kmp_rewrite (I 2 ⊗ hadamard) (I 2) ∣ 1 , 0 ⟩ ∣ 1 ⟩.
+  Msimpl'; trivial.
+  autorewrite with ket_db C_db.  
+  kmp_rewrite cnot (I 2) ∣ 0 , 1 ⟩ ∣ 1 ⟩.
+  kmp_rewrite cnot (I 2) ∣ 1 , 0 ⟩ ∣ 0 ⟩.
+  kmp_rewrite cnot (I 2) ∣ 1 , 1 ⟩ ∣ 1 ⟩.
+  
+  Msimpl'; try reflexivity.
+  autorewrite with ket_db.
+  
+
+  intros ψ ψ' WF H.
+  destruct_seqs; destruct_apps.
+  evar (e : Vector (2^3)).
+  assert ((ueval 3 U_H [a] × (ueval 3 U_CNOT (q::[a]) × (ueval 3 U_CNOT (a::[b]) × (ueval 3 U_H [a] × (ψ ⊗ ∣ 0, 0 ⟩))))) = e).
+  unfold ueval, ueval_cnot, ueval1, pad; simpl; Msimpl.
+  setoid_rewrite cnot_decomposition.
+  setoid_rewrite kron_assoc.
+  kmp_rewrite (I 2) (hadamard ⊗ I 2) ψ (∣ 0, 0 ⟩).
+  simpl in *; autorewrite with ket_db; trivial. (* autorewrite should discharge WF conditions! *)
+  idtac.                                                                                         
+  kmp_rewrite hadamard (I 2) ∣ 0 ⟩ ∣ 0 ⟩.
+  simpl in *; autorewrite with ket_db; auto with wf_db. (* autorewrite should discharge WF conditions! *)
+  Msimpl'.
+  simpl in *; autorewrite with ket_db; trivial. 
+  setoid_rewrite CNOT00_spec.
+  setoid_rewrite CNOT10_spec.
+  setoid_rewrite <- (kron_assoc _ _ _ _ _ _ ψ ∣ 0 ⟩ ∣ 0 ⟩).
+  setoid_rewrite <- (kron_assoc _ _ _ _ _ _ ψ ∣ 1 ⟩ ∣ 1 ⟩).
+  simpl in *; autorewrite with ket_db; trivial. 
+  kmp_rewrite cnot (I 2) (ψ ⊗ ∣ 0 ⟩) ∣ 0 ⟩.
+  kmp_rewrite cnot (I 2) (ψ ⊗ ∣ 1 ⟩) ∣ 1 ⟩.
+  Msimpl. 
+  setoid_rewrite <- (kron_assoc _ _ _ _ _ _ (I 2) hadamard (I 2)).
+  kmp_rewrite (I 2 ⊗ hadamard) (I 2) (cnot × (ψ ⊗ ∣ 0 ⟩)) ∣ 0 ⟩.  
+  kmp_rewrite (I 2 ⊗ hadamard) (I 2) (cnot × (ψ ⊗ ∣ 1 ⟩)) ∣ 1 ⟩.  
+  Msimpl.
+  unfold e. reflexivity.
+  dependent destruction H0_2.
+  inversion H0_2; subst.
+  
+  
+  
+  inversion H0_2.
+  unfold teleport in *.
+  match goal with
+  | [H : (_ ; _) / _ ⇩ _ |- _] => dependent destruction H
+  end.
+  
+  dependent destruction H.
+  dependent destruction H.
+  (* Bell State *)
+  assert ( ψ' = ψ ⊗ epr00).
+  dependent destruction H.
+  dependent destruction H.
+  dependent destruction H0.
+  
+  
+  replace (SQIMP.H a; CNOT a b) with (from_ucom (SQIMP.H a; CNOT a b))%ucom in H by reflexivity.
+  apply nd_eval_ucom in H; auto with wf_db.
+  simpl in H.
+  
+
+Lemma teleport_correct_manual : forall (ψ : Vector (2^1)) (ψ' : Vector (2^3)),
+  WF_Matrix _ _ ψ ->
+  teleport / (ψ  ⊗ ∣ 0 , 0 ⟩) ⇩ ψ' -> ψ' = ∣ 0 , 0 ⟩ ⊗ ψ.   
+Proof.
+  intros ψ ψ' WF H.
+  dependent destruction H.
+  dependent destruction H.
+  (* Bell State *)
+  assert ( ψ' = ψ ⊗ epr00).
+  dependent destruction H.
+  dependent destruction H.
+  dependent destruction H0.
+  simpl.
+  unfold ueval_cnot, ueval1, pad; simpl; Msimpl.
+  setoid_rewrite kron_assoc.
+  simpl.
+  kmp_rewrite (I 2) (hadamard ⊗ I 2) ψ (∣ 0, 0 ⟩).
+  kmp_rewrite hadamard (I 2) ∣0⟩ ∣0⟩. 
+  Msimpl.
+  setoid_rewrite H0_spec.  
+  kmp_rewrite (I 2) (∣1⟩⟨1∣ ⊗ σx .+ ∣0⟩⟨0∣ ⊗ I 2) ψ ((/ √ 2 .* ∣ 0 ⟩ .+ / √ 2 .* ∣ 1 ⟩) ⊗ ∣0⟩). 
+  Msimpl.                                                                                              
+  setoid_rewrite cnot_decomposition.
+  rewrite kron_plus_distr_r.
+  replace qubit0 with (ket 0) by reflexivity.
+  repeat rewrite Mscale_kron_dist_l.
+  rewrite Mmult_plus_distr_l.
+  repeat rewrite Mscale_mult_dist_r.
+  setoid_rewrite CNOT00_spec.
+  setoid_rewrite CNOT10_spec.
+  reflexivity.
+  (* Teleport *)
+  subst.
+  dependent destruction H0.
+  dependent destruction H0_.
+  
+  
+  Search scale Mmult.
+  Search cnot.
+  Search Mmult Mplus.
+  Search kron Mplus.
+  
+  rewrite Mmult_plus_dist_r.
+  replace (∣1⟩⟨1∣ ⊗ σx .+ ∣0⟩⟨0∣ ⊗ I 2) with cnot by solve_matrix. (* should be a lemma *)
+  kmp_rewrite hadamard (I 2) ∣0⟩ ∣0⟩. 
+  rewrite (Mmult_1_l _ _ ∣0⟩); auto with wf_db.
+                                    Msimpl.
+kmp_rewrite hadamard (I 2) ∣0⟩ ∣0⟩. 
+  Msimpl'.                                                                                                                                                                                     
+  Msimpl.
+  
+  
+  apply nd_seq_assoc in H.
+  cbv [teleport] in H.
+  repeat rewrite 
+  unfold teleport in H, bell00 in H, alice, bob, teleport in *.
+  
+  
+  dependent destruction H.
+  dependent destruction H.
+  dependent destruction H.
+  inversion H; subst.
+  dependent destruction H.
+  dependent destruction H0.
+  
+  
+  
